Two changes.
  1. Moved definition of ty_antiq to Parse so that it will
     appear in the docs. Other changes arose.

  2. "Fixed" HolCheck so that it builds. Is this a
     difference between the std and expt kernels?
     The change swaps type variables in arguments to
     type operators so is probably not what Hasan had
     in mind.

src/0/HolKernel.sml
@@ -13,20 +13,6 @@ infixr -->;  infix |->;
 val ERR = mk_HOL_ERR "HolKernel";
 
 (*---------------------------------------------------------------------------
-       Type antiquotations (required in term parser)
- ---------------------------------------------------------------------------*)
-
-fun ty_antiq ty = mk_var("ty_antiq",ty)
-
-fun dest_ty_antiq tm =
-  case with_exn dest_var tm (ERR "dest_ty_antiq" "not a type antiquotation")
-   of ("ty_antiq",Ty) => Ty
-    |  _ => raise ERR "dest_ty_antiq" "not a type antiquotation";
-
-val is_ty_antiq = Lib.can dest_ty_antiq
-
-
-(*---------------------------------------------------------------------------
           General term operations
  ---------------------------------------------------------------------------*)
 
