src/parse/term_pp.sig
@@ -5,6 +5,9 @@ sig
     term_grammar.grammar -> type_grammar.grammar -> Portable.ppstream ->
     Term.term -> unit
 
-end;
+  val ty_antiq      : Type.hol_type -> Term.term
+  val dest_ty_antiq : Term.term -> Type.hol_type
+  val is_ty_antiq   : Term.term -> bool
 
+end
 
