src/HolCheck/decompScript.sml
@@ -24,14 +24,14 @@ val AP_EXT = save_thm("AP_EXT",prove(list_mk_forall ([``f:'prop mu``,``ks1:('sta
 list_mk_imp([
 ``wfKS (ks1:('state1,'prop) KS)``,
 ``wfKS (ks2:('state2,'prop) KS)``,
-``!p (s1:'state1) (s2:'state2). p IN ks1.ap ==> (p IN (ks1:('prop,'state1) KS).L s1 = p IN (ks2:('prop,'state2) KS).L s2)``,
-``!a s1 s1' s2 s2'. ((s1>--(ks1:('prop,'state1) KS)/a-->s1' = s2>--(ks2:('prop,'state2) KS)/a-->s2'))``,
+``!p (s1:'state1) (s2:'state2). p IN ks1.ap ==> (p IN (ks1:('state1,'prop) KS).L s1 = p IN (ks2:('state2,'prop) KS).L s2)``,
+``!a s1 s1' s2 s2'. ((s1>--(ks1:('state1,'prop) KS)/a-->s1' = s2>--(ks2:('state2,'prop) KS)/a-->s2'))``,
 mk_forall(``Q:string``,mk_pforall(``s1:'state1``,mk_forall(``s2:'state2``,
 					      ``s1 IN ((e:string -> 'state1 -> bool) Q) = s2 IN ((e':string -> 'state2 -> bool) Q)``))),
 ``IMF (f:'prop mu)``,
-``!p. SUBFORMULA (AP p) f ==> p IN (ks1:('prop,'state1) KS).ap``
+``!p. SUBFORMULA (AP p) f ==> p IN (ks1:('state1,'prop) KS).ap``
 ],
-``(s1 IN STATES (f:'prop mu) (ks1:('prop,'state1) KS) (e:string -> 'state1 -> bool) = s2 IN STATES f (ks2:('prop,'state2) KS) (e':string -> 'state2 -> bool))``)),
+``(s1 IN STATES (f:'prop mu) (ks1:('state1,'prop) KS) (e:string -> 'state1 -> bool) = s2 IN STATES f (ks2:('state2,'prop) KS) (e':string -> 'state2 -> bool))``)),
 Induct_on `f` THEN REPEAT CONJ_TAC THENL [
 SIMP_TAC std_ss [STATES_def,IN_UNIV,wfKS_def], (* T *)
 SIMP_TAC std_ss [STATES_def, NOT_IN_EMPTY], (* F *)
@@ -85,11 +85,11 @@ REPEAT STRIP_TAC THENL [
 SIMP_TAC std_ss [STATES_def,SET_SPEC]
 THEN REPEAT STRIP_TAC
 THEN FULL_SIMP_TAC std_ss [SUB_AP_MU,IMF_def,STATES_def,SET_SPEC]
-THEN (SUBGOAL_THEN (list_mk_forall([``n:num``,``s1:'state1``,``s2:'state2``],``s1 IN FP f s (ks1:('prop,'state1) KS) e[[[s<--{}]]] n = s2 IN FP f s (ks2:('prop,'state2) KS) e'[[[s<--{}]]] n``)) ASSUME_TAC) THENL [
+THEN (SUBGOAL_THEN (list_mk_forall([``n:num``,``s1:'state1``,``s2:'state2``],``s1 IN FP f s (ks1:('state1,'prop) KS) e[[[s<--{}]]] n = s2 IN FP f s (ks2:('state2,'prop) KS) e'[[[s<--{}]]] n``)) ASSUME_TAC) THENL [
 Induct_on `n` THENL [
  RW_TAC std_ss [STATES_def,ENV_EVAL,NOT_IN_EMPTY], (* 0 *)
  REWRITE_TAC [STATES_def,ENV_UPDATE]
- THEN  (PAT_ASSUM ``!q1 q2 q3 q4 q5 q6. t`` (fn t => ASSUME_TAC (ISPECL [``(ks1:('prop,'state1) KS)``,``(ks2:('prop,'state2) KS)``,``e[[[s <-- FP f s (ks1:('prop,'state1) KS) e[[[s<--{}]]] n]]]``, ``e'[[[s<--FP f s (ks2:('prop,'state2) KS) e'[[[s<--{}]]] n]]]``] t)))
+ THEN  (PAT_ASSUM ``!q1 q2 q3 q4 q5 q6. t`` (fn t => ASSUME_TAC (ISPECL [``(ks1:('state1,'prop) KS)``,``(ks2:('state2,'prop) KS)``,``e[[[s <-- FP f s (ks1:('state1,'prop) KS) e[[[s<--{}]]] n]]]``, ``e'[[[s<--FP f s (ks2:('state2,'prop) KS) e'[[[s<--{}]]] n]]]``] t)))
   THEN RES_TAC
   THEN NTAC 2 (POP_ASSUM (K ALL_TAC))
   THEN POP_ASSUM (fn t => ASSUME_TAC t THEN SUBGOAL_THEN (fst(dest_imp(concl t))) ASSUME_TAC) THENL [
@@ -107,11 +107,11 @@ POP_ASSUM (fn t => METIS_TAC [t])
 SIMP_TAC std_ss [STATES_def,SET_SPEC]
 THEN REPEAT STRIP_TAC
 THEN FULL_SIMP_TAC std_ss [SUB_AP_NU,IMF_def]
-THEN (SUBGOAL_THEN (list_mk_forall([``n:num``,``s1:'state1``,``s2:'state2``],``s1 IN FP f s (ks1:('prop,'state1) KS) e[[[s<--ks1.S]]] n = s2 IN FP f s (ks2:('prop,'state2) KS) e'[[[s<--ks2.S]]] n``)) ASSUME_TAC) THENL [
+THEN (SUBGOAL_THEN (list_mk_forall([``n:num``,``s1:'state1``,``s2:'state2``],``s1 IN FP f s (ks1:('state1,'prop) KS) e[[[s<--ks1.S]]] n = s2 IN FP f s (ks2:('state2,'prop) KS) e'[[[s<--ks2.S]]] n``)) ASSUME_TAC) THENL [
 Induct_on `n` THENL [
   FULL_SIMP_TAC std_ss [STATES_def,ENV_EVAL,IN_UNIV,wfKS_def], (* 0 *)
   REWRITE_TAC [STATES_def,ENV_UPDATE]
-  THEN (PAT_ASSUM ``!q1 q2 q3 q4 q5 q6. t`` (fn t => ASSUME_TAC (ISPECL [``(ks1:('prop,'state1) KS)``,``(ks2:('prop,'state2) KS)``,``e[[[s <-- FP f s (ks1:('prop,'state1) KS) e[[[s<--ks1.S]]] n]]]``, ``e'[[[s<--FP f s (ks2:('prop,'state2) KS) e'[[[s<--ks2.S]]] n]]]``] t)))
+  THEN (PAT_ASSUM ``!q1 q2 q3 q4 q5 q6. t`` (fn t => ASSUME_TAC (ISPECL [``(ks1:('state1,'prop) KS)``,``(ks2:('state2,'prop) KS)``,``e[[[s <-- FP f s (ks1:('state1,'prop) KS) e[[[s<--ks1.S]]] n]]]``, ``e'[[[s<--FP f s (ks2:('state2,'prop) KS) e'[[[s<--ks2.S]]] n]]]``] t)))
   THEN RES_TAC
   THEN NTAC 2 (POP_ASSUM (K ALL_TAC))
   THEN POP_ASSUM (fn t => ASSUME_TAC t THEN SUBGOAL_THEN (fst(dest_imp(concl t))) ASSUME_TAC) THENL [
@@ -128,10 +128,10 @@ POP_ASSUM (fn t => METIS_TAC [t])
 ] (* nu *)
 ]));
 
-val lem3a = REWRITE_RULE [GSYM IMF_MU_NNF] (ISPECL [``ks:('prop,'state) KS``,``(NNF f):'prop mu``,``e:string->'state->bool``,``Y:'state->bool``,``X:'state->bool``,``Q:string``] (REWRITE_RULE [SUBSET_DEF] (GEN_ALL (SIMP_RULE std_ss [] (REWRITE_RULE [SUBSET_REFL] (ISPECL [``f:'prop mu``,``ks:('prop,'state) KS``,``e:string -> 'state -> bool``,``e:string -> 'state -> bool``,``Q:string``,``X:'state->bool``,``Y:'state->bool``] STATES_MONO))))));
+val lem3a = REWRITE_RULE [GSYM IMF_MU_NNF] (ISPECL [``ks:('state,'prop) KS``,``(NNF f):'prop mu``,``e:string->'state->bool``,``Y:'state->bool``,``X:'state->bool``,``Q:string``] (REWRITE_RULE [SUBSET_DEF] (GEN_ALL (SIMP_RULE std_ss [] (REWRITE_RULE [SUBSET_REFL] (ISPECL [``f:'prop mu``,``ks:('state,'prop) KS``,``e:string -> 'state -> bool``,``e:string -> 'state -> bool``,``Q:string``,``X:'state->bool``,``Y:'state->bool``] STATES_MONO))))));
 
 (* gen decomp proof *)
-val DECOMP = save_thm("DECOMP",SIMP_RULE std_ss [STATES_NNF_ID] (prove(list_mk_pforall ([``(f:'prop mu)``,``s:'state``,``(e:string -> 'state -> bool)``,``Q:string``,``ks1:('prop,'state) KS``,``ks2:('prop,'state) KS``],list_mk_imp([``IMF mu (Q:string) .. (f:'prop mu)``,``!a g. ~SUBFORMULA (<<a>> g) (NNF (f:'prop mu))``,``wfKS (ks1:('prop,'state) KS)``,``wfKS (ks2:('prop,'state) KS)``,``(ks1:('prop,'state) KS).ap=(ks2:('prop,'state) KS).ap``,``(ks1:('prop,'state) KS).L=(ks2:('prop,'state) KS).L``,``!a s s'. ((ks2:('prop,'state) KS).T a)(s,s') ==> ((ks1:('prop,'state) KS).T a)(s,s')``],``s IN STATES (NNF (f:'prop mu)) (ks1:('prop,'state) KS) e ==> s IN STATES (NNF f) (ks2:('prop,'state) KS) e``)),
+val DECOMP = save_thm("DECOMP",SIMP_RULE std_ss [STATES_NNF_ID] (prove(list_mk_pforall ([``(f:'prop mu)``,``s:'state``,``(e:string -> 'state -> bool)``,``Q:string``,``ks1:('state,'prop) KS``,``ks2:('state,'prop) KS``],list_mk_imp([``IMF mu (Q:string) .. (f:'prop mu)``,``!a g. ~SUBFORMULA (<<a>> g) (NNF (f:'prop mu))``,``wfKS (ks1:('state,'prop) KS)``,``wfKS (ks2:('state,'prop) KS)``,``(ks1:('state,'prop) KS).ap=(ks2:('state,'prop) KS).ap``,``(ks1:('state,'prop) KS).L=(ks2:('state,'prop) KS).L``,``!a s s'. ((ks2:('state,'prop) KS).T a)(s,s') ==> ((ks1:('state,'prop) KS).T a)(s,s')``],``s IN STATES (NNF (f:'prop mu)) (ks1:('state,'prop) KS) e ==> s IN STATES (NNF f) (ks2:('state,'prop) KS) e``)),
 recInduct NNF_IND_def THEN REPEAT CONJ_TAC THENL [
 SIMP_TAC std_ss [NNF_def,STATES_def,wfKS_def,IN_UNIV], (* T *)
 SIMP_TAC std_ss [NNF_def,STATES_def], (* F *)
@@ -155,13 +155,13 @@ THEN NTAC 15 STRIP_TAC
 THEN IMP_RES_TAC IMF_MU_MU
 THEN FULL_SIMP_TAC std_ss [SUB_DMD_MU]
 THEN RES_TAC
-THEN (SUBGOAL_THEN (mk_forall(``n:num``,list_mk_forall([``s:'state``],mk_imp(``s IN FP (NNF f) Q (ks1:('prop,'state) KS) e[[[Q<--{}]]] n``,``s IN FP (NNF f) Q (ks2:('prop,'state) KS) e[[[Q<--{}]]] n``)))) ASSUME_TAC) THENL [
+THEN (SUBGOAL_THEN (mk_forall(``n:num``,list_mk_forall([``s:'state``],mk_imp(``s IN FP (NNF f) Q (ks1:('state,'prop) KS) e[[[Q<--{}]]] n``,``s IN FP (NNF f) Q (ks2:('state,'prop) KS) e[[[Q<--{}]]] n``)))) ASSUME_TAC) THENL [
  Induct_on `n` THENL [
   SIMP_TAC std_ss [STATES_def,ENV_EVAL],
   SIMP_TAC std_ss [STATES_def,ENV_UPDATE]
   THEN POP_ASSUM (fn t => ASSUME_TAC t THEN UNDISCH_TAC (concl t))
-  THEN SPEC_TAC (``FP (NNF f) Q  (ks1:('prop,'state) KS) e[[[Q<--{}]]] n``,``X:'state -> bool``)
-  THEN SPEC_TAC (``FP (NNF f) Q  (ks2:('prop,'state) KS)e[[[Q<--{}]]] n``,``Y:'state->bool``)
+  THEN SPEC_TAC (``FP (NNF f) Q  (ks1:('state,'prop) KS) e[[[Q<--{}]]] n``,``X:'state -> bool``)
+  THEN SPEC_TAC (``FP (NNF f) Q  (ks2:('state,'prop) KS)e[[[Q<--{}]]] n``,``Y:'state->bool``)
   THEN REPEAT GEN_TAC
   THEN STRIP_TAC
   THEN IMP_RES_TAC lem3a
@@ -174,14 +174,14 @@ THEN NTAC 15 STRIP_TAC
 THEN IMP_RES_TAC IMF_MU_NU
 THEN FULL_SIMP_TAC std_ss [SUB_DMD_NU]
 THEN RES_TAC
-THEN (SUBGOAL_THEN (mk_forall(``n:num``,mk_forall(``s:'state``,mk_imp(``s IN FP (NNF f) Q (ks1:('prop,'state) KS) e[[[Q<--ks1.S]]] n``,``s IN FP (NNF f) Q (ks2:('prop,'state) KS) e[[[Q<--ks2.S]]] n``)))) ASSUME_TAC) THENL [
+THEN (SUBGOAL_THEN (mk_forall(``n:num``,mk_forall(``s:'state``,mk_imp(``s IN FP (NNF f) Q (ks1:('state,'prop) KS) e[[[Q<--ks1.S]]] n``,``s IN FP (NNF f) Q (ks2:('state,'prop) KS) e[[[Q<--ks2.S]]] n``)))) ASSUME_TAC) THENL [
  Induct_on `n` THENL [
   SIMP_TAC std_ss [STATES_def,ENV_EVAL]
   THEN FULL_SIMP_TAC std_ss [wfKS_def],
   SIMP_TAC std_ss [STATES_def,ENV_UPDATE]
   THEN POP_ASSUM (fn t => ASSUME_TAC t THEN UNDISCH_TAC (concl t))
-  THEN SPEC_TAC (``FP (NNF f) Q (ks1:('prop,'state) KS) e[[[Q<--ks1.S]]] n``,``X:'state -> bool``)
-  THEN SPEC_TAC (``FP (NNF f) Q (ks2:('prop,'state) KS) e[[[Q<--ks2.S]]] n``,``Y:'state ->bool``)
+  THEN SPEC_TAC (``FP (NNF f) Q (ks1:('state,'prop) KS) e[[[Q<--ks1.S]]] n``,``X:'state -> bool``)
+  THEN SPEC_TAC (``FP (NNF f) Q (ks2:('state,'prop) KS) e[[[Q<--ks2.S]]] n``,``Y:'state ->bool``)
   THEN REPEAT GEN_TAC
   THEN STRIP_TAC
   THEN IMP_RES_TAC lem3a
@@ -213,13 +213,13 @@ THEN IMP_RES_TAC IMF_MU_NEG_MU
 THEN FULL_SIMP_TAC std_ss [SUB_DMD_NU]
 THEN POP_ASSUM (fn t => ASSUME_TAC (ONCE_REWRITE_RULE [IMF_MU_INV_RVNEG] t))
 THEN RES_TAC
-THEN (SUBGOAL_THEN (mk_forall(``n:num``,mk_forall(``s:'state``,mk_imp(``s IN FP (NNF (RVNEG Q ~f)) Q (ks1:('prop,'state) KS) e[[[Q<--ks1.S]]] n``,``s IN FP (NNF (RVNEG Q ~f)) Q (ks2:('prop,'state) KS) e[[[Q<--ks2.S]]] n``)))) ASSUME_TAC) THENL [
+THEN (SUBGOAL_THEN (mk_forall(``n:num``,mk_forall(``s:'state``,mk_imp(``s IN FP (NNF (RVNEG Q ~f)) Q (ks1:('state,'prop) KS) e[[[Q<--ks1.S]]] n``,``s IN FP (NNF (RVNEG Q ~f)) Q (ks2:('state,'prop) KS) e[[[Q<--ks2.S]]] n``)))) ASSUME_TAC) THENL [
  Induct_on `n` THENL [
   FULL_SIMP_TAC std_ss [STATES_def,ENV_EVAL,wfKS_def],
   SIMP_TAC std_ss [STATES_def,ENV_UPDATE]
   THEN POP_ASSUM (fn t => ASSUME_TAC t THEN UNDISCH_TAC (concl t))
-  THEN SPEC_TAC (``FP (NNF (RVNEG Q ~f)) Q (ks1:('prop,'state) KS) e[[[Q<--ks1.S]]] n``,``X:'state -> bool``)
-  THEN SPEC_TAC (``FP (NNF (RVNEG Q ~f)) Q (ks2:('prop,'state) KS) e[[[Q<--ks2.S]]] n``,``Y:'state->bool``)
+  THEN SPEC_TAC (``FP (NNF (RVNEG Q ~f)) Q (ks1:('state,'prop) KS) e[[[Q<--ks1.S]]] n``,``X:'state -> bool``)
+  THEN SPEC_TAC (``FP (NNF (RVNEG Q ~f)) Q (ks2:('state,'prop) KS) e[[[Q<--ks2.S]]] n``,``Y:'state->bool``)
   THEN REPEAT GEN_TAC
   THEN STRIP_TAC
   THEN IMP_RES_TAC lem3a
@@ -233,13 +233,13 @@ THEN IMP_RES_TAC IMF_MU_NEG_NU
 THEN FULL_SIMP_TAC std_ss [SUB_DMD_MU]
 THEN POP_ASSUM (fn t => ASSUME_TAC (ONCE_REWRITE_RULE [IMF_MU_INV_RVNEG] t))
 THEN RES_TAC
-THEN (SUBGOAL_THEN (mk_forall(``n:num``,mk_forall(``s:'state``,mk_imp(``s IN FP (NNF (RVNEG Q ~f)) Q (ks1:('prop,'state) KS) e[[[Q<--{}]]] n``,``s IN FP (NNF (RVNEG Q ~f)) Q (ks2:('prop,'state) KS) e[[[Q<--{}]]] n``)))) ASSUME_TAC) THENL [
+THEN (SUBGOAL_THEN (mk_forall(``n:num``,mk_forall(``s:'state``,mk_imp(``s IN FP (NNF (RVNEG Q ~f)) Q (ks1:('state,'prop) KS) e[[[Q<--{}]]] n``,``s IN FP (NNF (RVNEG Q ~f)) Q (ks2:('state,'prop) KS) e[[[Q<--{}]]] n``)))) ASSUME_TAC) THENL [
  Induct_on `n` THENL [
   SIMP_TAC std_ss [STATES_def,ENV_EVAL],
   SIMP_TAC std_ss [STATES_def,ENV_UPDATE]
   THEN POP_ASSUM (fn t => ASSUME_TAC t THEN UNDISCH_TAC (concl t))
-  THEN SPEC_TAC (``FP (NNF (RVNEG Q ~f)) Q (ks1:('prop,'state) KS) e[[[Q<--{}]]] n``,``X:'state -> bool``)
-  THEN SPEC_TAC (``FP (NNF (RVNEG Q ~f)) Q (ks2:('prop,'state) KS) e[[[Q<--{}]]] n``,``Y:'state ->bool``)
+  THEN SPEC_TAC (``FP (NNF (RVNEG Q ~f)) Q (ks1:('state,'prop) KS) e[[[Q<--{}]]] n``,``X:'state -> bool``)
+  THEN SPEC_TAC (``FP (NNF (RVNEG Q ~f)) Q (ks2:('state,'prop) KS) e[[[Q<--{}]]] n``,``Y:'state ->bool``)
   THEN REPEAT GEN_TAC
   THEN STRIP_TAC
   THEN IMP_RES_TAC lem3a
